Lean4Lean/Theory.lean
@@ -6,3 +6,4 @@ import Lean4Lean.Theory.Typing.ChurchRosser
 import Lean4Lean.Theory.Typing.HeadReduction
 import Lean4Lean.Theory.LocalContext
 import Lean4Lean.Theory.Literals
+import Lean4Lean.Theory.Projection
